More faithful copy of Isabelle sem

bot/intervalArithScript.sml
@@ -1,10 +1,14 @@
 open preamble
+open blastLib
 
 val _ = new_theory "intervalArith";
 
 (*
   Define a copy of the word arithmetic semantics
   from the Isabelle/HOL formalization
+
+  NOTE: the Isabelle semantics removes the constant 0x80000000
+  from the word32 type, which we omit here
 *)
 
 val NEG_INF = (rconc o EVAL) ``((INT_MINw: 32 word) + 1w)``
@@ -13,20 +17,15 @@ val POS_INF = (rconc o EVAL) ``((INT_MAXw: 32 word) )``
 val NEG_INF_def = Define`NEG_INF:word32 = ^NEG_INF`
 val POS_INF_def = Define`POS_INF:word32 = ^POS_INF`
 
-(*
-  Note: this includes the constant INT_MINw which is interpreted as the interval
-  (-INF,INF)
-  All other constants are interpreted as in the Isabelle formalization e.g.
-  -INF is interpreted as (-INF,-INF)
-*)
 val _ = Datatype`
   trm = Const word32
-      | Var string (* TODO: this could also use the faster mlstring *)
+      | Var string
       | Plus trm trm
       | Times trm trm
       | Max trm trm
       | Min trm trm
-      | Neg trm`
+      | Neg trm
+      | Abs trm`
 
 val _ = Datatype`
   fml = Le trm trm
@@ -36,7 +35,6 @@ val _ = Datatype`
       | Or fml fml
       | Not fml`
 
-(* The discrete fragment of hybrid programs we need for sandboxes *)
 val _ = Datatype`
    hp = Test fml
       | Assign string (trm option)
@@ -45,64 +43,84 @@ val _ = Datatype`
       | Loop hp
       | Skip`
 
-val round_to_inf_def = Define`
-  round_to_inf (w:word64) =
-    if w ≤ sw2sw NEG_INF then NEG_INF
-    else if
-      sw2sw POS_INF ≤ w then POS_INF
-    else
-      w2w w`
-
+(* First, define the helper functions following Isabelle formalization
+  We will simplify these later *)
 val pu_def = Define`
   pu (w1:word32) (w2:word32) =
-  if w1 = POS_INF ∨ w2 = POS_INF
-  then POS_INF
+  if w1 = POS_INF then POS_INF
+  else if w2 = POS_INF then POS_INF
+  else if w1 = NEG_INF then
+    (if w2 = NEG_INF then NEG_INF
+    else
+      let sum:word64 = sw2sw w2 + sw2sw NEG_INF in
+      if sum ≤ sw2sw NEG_INF then NEG_INF
+      else sw2sw sum)
+  else if w2 = NEG_INF then
+    let sum:word64 = sw2sw w1 +sw2sw NEG_INF in
+    if sum ≤ sw2sw NEG_INF then NEG_INF
+    else sw2sw sum
   else
-    let s:word64 = sw2sw w1 + sw2sw w2 in
-    round_to_inf s`
+    let sum:word64 = sw2sw w1 + sw2sw w2 in
+    if sw2sw POS_INF ≤ sum then POS_INF
+    else if sum ≤ sw2sw NEG_INF then NEG_INF
+    else sw2sw sum`
 
 val pl_def = Define`
   pl (w1:word32) (w2:word32) =
-  if w1 = NEG_INF ∨ w2 = NEG_INF then NEG_INF
+  if w1 = NEG_INF then NEG_INF
+  else if w2 = NEG_INF then NEG_INF
+  else if w1 = POS_INF then
+    (if w2 = POS_INF then POS_INF
+    else
+      let sum:word64 = sw2sw w2 + sw2sw POS_INF in
+      if sw2sw POS_INF ≤ sum then POS_INF
+      else sw2sw sum)
+  else if w2 = NEG_INF then
+    let sum:word64 = sw2sw w1 + sw2sw POS_INF in
+    if sw2sw POS_INF ≤ sum then POS_INF
+    else sw2sw sum
   else
-  let s:word64 = sw2sw w1 + sw2sw w2 in
-  round_to_inf s`
+    let sum:word64 = sw2sw w1 + sw2sw w2 in
+    if sw2sw POS_INF ≤ sum then POS_INF
+    else if sum ≤ sw2sw NEG_INF then NEG_INF
+    else sw2sw sum`
+
+val wtimes_def = Define`
+  wtimes (w1:word32) (w2:word32) =
+  if w1 = POS_INF ∧ w2 = POS_INF then POS_INF
+  else if w1 = NEG_INF ∧ w2 = POS_INF then NEG_INF
+  else if w1 = POS_INF ∧ w2 = NEG_INF then NEG_INF
+  else if w1 = NEG_INF ∧ w2 = NEG_INF then POS_INF
+
+  else if w1 = POS_INF ∧ w2 < 0w then NEG_INF
+  else if w1 = POS_INF ∧ 0w < w2 then POS_INF
+  else if w1 = POS_INF ∧ 0w = w2 then 0w
+  else if w1 = NEG_INF ∧ w2 < 0w then POS_INF
+  else if w1 = NEG_INF ∧ 0w < w2 then NEG_INF
+  else if w1 = NEG_INF ∧ 0w = w2 then 0w
+
+  else if w1 < 0w ∧ w2 = POS_INF then NEG_INF
+  else if 0w < w1 ∧ w2 = POS_INF then POS_INF
+  else if 0w = w1 ∧ w2 = POS_INF then 0w
+  else if w1 < 0w ∧ w2 = NEG_INF then POS_INF
+  else if 0w < w1 ∧ w2 = NEG_INF then NEG_INF
+  else if 0w = w1 ∧ w2 = NEG_INF then 0w
+  else
+  let prod:word64 = sw2sw w1 * sw2sw w2 in
+  if prod ≤ sw2sw NEG_INF then NEG_INF
+  else if sw2sw POS_INF ≤ prod then POS_INF
+  else sw2sw prod`
 
 val wmax_def = Define`
   wmax (w1:word32) (w2:word32) = if w1 < w2 then w2 else w1`
 
-val wtimes_def = Define`
-  wtimes (w1:word32) (w2:word32) =
-  let prod = sw2sw w1 * sw2sw w2 in round_to_inf prod`
-
-(* Checking the simplification
-EVAL``wtimes POS_INF POS_INF = POS_INF``
-EVAL``wtimes NEG_INF POS_INF = NEG_INF``
-EVAL``wtimes POS_INF NEG_INF = NEG_INF``
-EVAL``wtimes NEG_INF NEG_INF = POS_INF``
-
-EVAL``wtimes POS_INF (-1w) = NEG_INF``
-EVAL``wtimes POS_INF (1w) = POS_INF``
-EVAL``wtimes POS_INF 0w = 0w``
-EVAL``wtimes NEG_INF (-1w) = POS_INF``
-EVAL``wtimes NEG_INF (1w) = NEG_INF``
-EVAL``wtimes NEG_INF 0w = 0w``
-
-EVAL``wtimes (-1w) POS_INF = NEG_INF``
-EVAL``wtimes (1w) POS_INF = POS_INF``
-EVAL``wtimes 0w POS_INF = 0w``
-EVAL``wtimes (-1w) NEG_INF = POS_INF``
-EVAL``wtimes (1w) NEG_INF = NEG_INF``
-EVAL``wtimes 0w NEG_INF = 0w``
-*)
+val wmin_def = Define`
+  wmin (w1:word32) (w2:word32) = if w1 < w2 then w1 else w2`
 
 val tu_def = Define`
   tu w1l w1u w2l w2u =
   wmax (wmax (wtimes w1l w2l) (wtimes w1u w2l))
        (wmax (wtimes w1l w2u) (wtimes w1u w2u))`
-
-val wmin_def = Define`
-  wmin (w1:word32) (w2:word32) = if w1 < w2 then w1 else w2`
 
 val tl_def = Define`
   tl w1l w1u w2l w2u =
@@ -115,28 +133,13 @@ val wneg_def = Define`
   else if w = POS_INF then NEG_INF
   else -w`;
 
-(* States are represented as an association list of
-  strings -> (w32,w32) *)
-val _ = type_abbrev ("wstate",``:(string,word32 # word32) alist``)
-
-(* Differences from Isabelle formalization:
-   The state is a finite map -- when Var n is not in the map, we assume that
-   it is in the interval (-Inf,Inf)
-*)
-val lookup_const_def = Define`
-  lookup_const w =
-     if NEG_INF ≤ w ∧ w ≤ POS_INF then (w,w)
-     else (NEG_INF,POS_INF)`
-
-val lookup_var_def = Define`
-  lookup_var s n =
-    case ALOOKUP s n of
-      NONE => (NEG_INF,POS_INF)
-    | SOME i => i`
+(* Following the Isabelle semantics, we first use abstract word states
+   that map a sum to words *)
+val _ = type_abbrev ("wstate",``:string+string -> word32``);
 
 val wtsem_def = Define`
-  (wtsem (Const w) (s:wstate) = lookup_const w) ∧
-  (wtsem (Var n) s = lookup_var s n) ∧
+  (wtsem (Const r) (s:wstate) = (r,r)) ∧
+  (wtsem (Var x) s = (s (INL x), s (INR x))) ∧
   (wtsem (Plus t1 t2) s =
     let (l1,u1) = wtsem t1 s in
     let (l2,u2) = wtsem t2 s in
@@ -155,7 +158,10 @@ val wtsem_def = Define`
     (wmin l1 l2, wmin u1 u2)) ∧
   (wtsem (Neg t) s =
     let (l,u) = wtsem t s in
-    (wneg u, wneg l))`
+    (wneg u, wneg l)) ∧
+  (wtsem (Abs t) s =
+    let (l,u) = wtsem t s in
+    (wmax l (wneg u), wmax u (wneg l)))`
 
 val wle_def = Define`
   wle (w1:word32) w2 <=> w1 < w2`
@@ -166,76 +172,285 @@ val wleq_def = Define`
   ¬ (w2 = POS_INF ∧ w2 = POS_INF) ∧
   w1 <= w2`
 
-(* We use a tri-valued logic for wfsem instead of an underspecified relation *)
+val (wfsem_rules,wfsem_ind, wfsem_cases) = Hol_reln`
+  (∀t1 t2 s.
+    wle (SND (wtsem t1 s)) (FST (wtsem t2 s)) ⇒
+    wfsem (Le t1 t2) s T) ∧
+  (∀t1 t2 s.
+    wleq (SND (wtsem t2 s)) (FST (wtsem t1 s)) ⇒
+    wfsem (Le t1 t2) s F) ∧
+  (∀t1 t2 s.
+    wleq (SND (wtsem t1 s)) (FST (wtsem t2 s)) ⇒
+    wfsem (Leq t1 t2) s T) ∧
+  (∀t1 t2 s.
+    wle (SND (wtsem t2 s)) (FST (wtsem t1 s)) ⇒
+    wfsem (Leq t1 t2) s F) ∧
+  (∀t1 t2 s.
+    FST (wtsem t2 s) = SND (wtsem t2 s) ∧
+    SND (wtsem t2 s) = SND (wtsem t1 s) ∧
+    SND (wtsem t1 s) = FST (wtsem t1 s) ∧
+    FST (wtsem t2 s) ≠ NEG_INF ∧
+    FST (wtsem t2 s) ≠ POS_INF ⇒
+    wfsem (Equals t1 t2) s T) ∧
+  (∀t1 t2 s.
+    wle (SND (wtsem t1 s)) (FST (wtsem t2 s)) ⇒
+    wfsem (Equals t1 t2) s F) ∧
+  (∀t1 t2 s.
+    wle (SND (wtsem t2 s)) (FST (wtsem t1 s)) ⇒
+    wfsem (Equals t1 t2) s F) ∧
+  (∀f1 f2 s.
+    wfsem f1 s T ∧
+    wfsem f2 s T ⇒
+    wfsem (And f1 f2) s T) ∧
+  (∀f1 f2 s.
+    wfsem f1 s F ⇒
+    wfsem (And f1 f2) s F) ∧
+  (∀f1 f2 s.
+    wfsem f2 s F ⇒
+    wfsem (And f1 f2) s F) ∧
+  (∀f1 f2 s.
+    wfsem f1 s T ⇒
+    wfsem (Or f1 f2) s T) ∧
+  (∀f1 f2 s.
+    wfsem f2 s T ⇒
+    wfsem (Or f1 f2) s T) ∧
+  (∀f1 f2 s.
+    wfsem f1 s F ∧
+    wfsem f1 s F ⇒
+    wfsem (Or f1 f2) s F) ∧
+  (∀f s.
+    wfsem f s F ⇒
+    wfsem (Not f) s T) ∧
+  (∀f s.
+    wfsem f s T ⇒
+    wfsem (Not f) s F)`
 
-val wfsem_def = Define`
-  (wfsem (Le t1 t2) (s:wstate) =
-  let (l1,u1) = wtsem t1 s in
-  let (l2,u2) = wtsem t2 s in
+(* The non-deterministic big-step relational semantics of hybrid programs *)
+val (wpsem_rules,wpsem_ind, wpsem_cases) = Hol_reln`
+  (* wTest *)
+  (∀f w v.
+    wfsem f w T ∧ v = w ⇒
+    wpsem (Test f) v w) ∧
+  (* wSeq *)
+  (∀a b w u v.
+    wpsem a v u ∧
+    wpsem b u w ⇒
+    wpsem (Seq a b) v w) ∧
+  (* wAssign *)
+  (∀x t w v.
+    (w = λy. if y = INR x then SND (wtsem t v)
+            else if y = INL x then FST (wtsem t v)
+            else v y) ⇒
+    wpsem (Assign x (SOME t)) v w) ∧
+  (* wChoice1 *)
+  (∀a b w v.
+    wpsem a v w ⇒
+    wpsem (Choice a b) v w) ∧
+  (* wChoice2 *)
+  (∀a b w v.
+    wpsem b v w ⇒
+    wpsem (Choice a b) v w) ∧
+  (* TODO: add these *)
+  (∀w. wpsem Skip w w) ∧
+  (* Non-deterministic assignment *)
+  (∀x a b w v.
+  a ≤ b ∧
+  (w = λy. if y = INR x then b
+            else if y = INL x then a
+            else v y) ⇒
+  wpsem (Assign x NONE) v w) ∧
+  (∀a w.
+    wpsem (Loop a) w w) ∧
+  (∀a w v u.
+    wpsem a v u ∧
+    wpsem (Loop a) u w ⇒
+    wpsem (Loop a) v w)`
+
+(* Now we define the actual semantics that we will work with
+  These operate over concrete word states
+*)
+val _ = type_abbrev ("cwstate",``:(string,word32 # word32) alist``)
+
+val lookup_var_def = Define`
+  lookup_var s n =
+    case ALOOKUP s n of
+      NONE => (NEG_INF,POS_INF)
+    | SOME i => i`
+
+(* abstract concrete cwstate back into a wstate *)
+val abs_state_def = Define`
+  abs_state (s:cwstate) =
+  λy.
+    case y of
+      INL x => FST (lookup_var s x)
+    | INR x => SND (lookup_var s x)`
+
+val cwtsem_def = Define`
+  (cwtsem (Const w) (s:cwstate) = (w,w)) ∧
+  (cwtsem (Var n) s = lookup_var s n) ∧
+  (cwtsem (Plus t1 t2) s =
+    let (l1,u1) = cwtsem t1 s in
+    let (l2,u2) = cwtsem t2 s in
+    (pl l1 l2, pu u1 u2)) ∧
+  (cwtsem (Times t1 t2) s =
+    let (l1,u1) = cwtsem t1 s in
+    let (l2,u2) = cwtsem t2 s in
+    (tl l1 u1 l2 u2, tu l1 u1 l2 u2)) ∧
+  (cwtsem (Max t1 t2) s =
+    let (l1,u1) = cwtsem t1 s in
+    let (l2,u2) = cwtsem t2 s in
+    (wmax l1 l2, wmax u1 u2)) ∧
+  (cwtsem (Min t1 t2) s =
+    let (l1,u1) = cwtsem t1 s in
+    let (l2,u2) = cwtsem t2 s in
+    (wmin l1 l2, wmin u1 u2)) ∧
+  (cwtsem (Neg t) s =
+    let (l,u) = cwtsem t s in
+    (wneg u, wneg l)) ∧
+  (cwtsem (Abs t) s =
+    let (l,u) = cwtsem t s in
+    (wmax l (wneg u), wmax u (wneg l)))`
+
+val cwtsem_wtsem = Q.store_thm("cwtsem_wtsem",`
+  ∀t cs s.
+ cwtsem t cs = wtsem t (abs_state cs)`,
+  Induct>>fs[cwtsem_def,wtsem_def,lookup_var_def,abs_state_def]);
+
+(* We use a tri-valued logic for wfsem instead of an underspecified relation *)
+val cwfsem_def = Define`
+  (cwfsem (Le t1 t2) (s:cwstate) =
+  let (l1,u1) = cwtsem t1 s in
+  let (l2,u2) = cwtsem t2 s in
   if wle u1 l2 then SOME T
   else if wleq u2 l1 then SOME F
   else NONE) ∧
-  (wfsem (Leq t1 t2) s =
-  let (l1,u1) = wtsem t1 s in
-  let (l2,u2) = wtsem t2 s in
+  (cwfsem (Leq t1 t2) s =
+  let (l1,u1) = cwtsem t1 s in
+  let (l2,u2) = cwtsem t2 s in
   if wleq u1 l2 then SOME T
   else if wle u2 l1 then SOME F
   else NONE) ∧
-  (wfsem (Equals t1 t2) s =
-  let (l1,u1) = wtsem t1 s in
-  let (l2,u2) = wtsem t2 s in
+  (cwfsem (Equals t1 t2) s =
+  let (l1,u1) = cwtsem t1 s in
+  let (l2,u2) = cwtsem t2 s in
   if l2 = u2 ∧ u2 = u1 ∧ u1 = l1 ∧ l2 ≠ NEG_INF ∧ l2 ≠ POS_INF then SOME T
   else if wle u1 l2 then SOME F
   else if wle u2 l1 then SOME F
   else NONE) ∧
-  (wfsem (And f1 f2) s =
-  case (wfsem f1 s, wfsem f2 s) of
+  (cwfsem (And f1 f2) s =
+  case (cwfsem f1 s, cwfsem f2 s) of
     SOME T, SOME T => SOME T
   | SOME F, _ => SOME F
   | _, SOME F => SOME F
   | _ => NONE) ∧
-  (wfsem (Or f1 f2) s =
-  case (wfsem f1 s, wfsem f2 s) of
+  (cwfsem (Or f1 f2) s =
+  case (cwfsem f1 s, cwfsem f2 s) of
     SOME T, _ => SOME T
   | _, SOME T => SOME T
   | SOME F, SOME F => SOME F
   | _ => NONE) ∧
-  (wfsem (Not f) s =
-  case wfsem f s of
+  (cwfsem (Not f) s =
+  case cwfsem f s of
     SOME F => SOME T
   | SOME T => SOME F
   | _ => NONE)`
 
+(* The reverse direction should also be true, but we do not need it *)
+val cwfsem_wfsem = Q.store_thm("cwfsem_wfsem",`
+  ∀f cs s b.
+  (cwfsem f cs = SOME b ⇒ wfsem f (abs_state cs) b)`,
+  Induct>>fs[cwfsem_def]>>rw[]>>
+  TRY
+    (rpt (pairarg_tac>>fs[])>>
+    EVERY_CASE_TAC>>fs[]>>
+    simp[Once wfsem_cases,GSYM cwtsem_wtsem])>>
+  rw[]);
+
 (* The non-deterministic big-step relational semantics of hybrid programs *)
-val (wpsem_rules,wpsem_ind, wpsem_cases) = Hol_reln`
+val (cwpsem_rules,cwpsem_ind, cwpsem_cases) = Hol_reln`
   (* skip *)
-  (∀w. wpsem Skip w w) ∧
+  (∀w. cwpsem Skip w w) ∧
   (* Non-deterministic assignment *)
   (∀x a b w.
   a ≤ b ⇒
-  wpsem (Assign x NONE) w ((x,(a,b))::w)) ∧
+  cwpsem (Assign x NONE) w ((x,(a,b))::w)) ∧
   (* Deterministic assignment *)
   (∀x t w.
-  wpsem (Assign x (SOME t)) w ((x,(wtsem t w))::w)) ∧
+  cwpsem (Assign x (SOME t)) w ((x,(cwtsem t w))::w)) ∧
   (∀f w.
-    wfsem f w = SOME T ⇒
-    wpsem (Test f) w w) ∧
+    cwfsem f w = SOME T ⇒
+    cwpsem (Test f) w w) ∧
   (∀a b w u v.
-    wpsem a w u ∧
-    wpsem b u v ⇒
-    wpsem (Seq a b) w v) ∧
+    cwpsem a w u ∧
+    cwpsem b u v ⇒
+    cwpsem (Seq a b) w v) ∧
   (∀a b w v.
-    wpsem a w v ⇒
-    wpsem (Choice a b) w v) ∧
+    cwpsem a w v ⇒
+    cwpsem (Choice a b) w v) ∧
   (∀a b w v.
-    wpsem b w v ⇒
-    wpsem (Choice a b) w v) ∧
+    cwpsem b w v ⇒
+    cwpsem (Choice a b) w v) ∧
   (∀a w.
-    wpsem (Loop a) w w) ∧
+    cwpsem (Loop a) w w) ∧
   (∀a w.
-    wpsem a w u ∧
-    wpsem (Loop a) u v ⇒
-    wpsem (Loop a) w v)`
+    cwpsem a w u ∧
+    cwpsem (Loop a) u v ⇒
+    cwpsem (Loop a) w v)`
+
+val cwpsem_wpsem = Q.store_thm("cwpsem_wpsem",`
+  ∀p w v.
+  cwpsem p w v ⇒ wpsem p (abs_state w) (abs_state v)`,
+  ho_match_mp_tac cwpsem_ind>>rw[]>>
+  simp[Once wpsem_cases,cwfsem_wfsem]
+  >-
+    (asm_exists_tac>>simp[abs_state_def]>>
+    simp[FUN_EQ_THM,lookup_var_def]>>
+    rw[]>>EVERY_CASE_TAC>>fs[])
+  >-
+    (simp[cwtsem_wtsem,abs_state_def]>>
+    simp[FUN_EQ_THM,lookup_var_def]>>
+    rw[]>>EVERY_CASE_TAC>>fs[])
+  >>
+    metis_tac[]);
+
+(* More efficient simplifications for the bounds checks *)
+val round_to_inf_def = Define`
+  round_to_inf (w:word64) =
+    if w ≤ sw2sw NEG_INF then NEG_INF
+    else if
+      sw2sw POS_INF ≤ w then POS_INF
+    else
+      w2w w`
+
+val pu_compute = Q.store_thm("pu_compute",`
+  pu (w1:word32) (w2:word32) =
+  if w1 = POS_INF ∨ w2 = POS_INF
+  then POS_INF
+  else
+    let s:word64 = sw2sw w1 + sw2sw w2 in
+    round_to_inf s`,
+  rw[pu_def]>>fs[round_to_inf_def]>>
+  rpt (pop_assum mp_tac)>> EVAL_TAC>>
+  rw[]>>
+  blastLib.FULL_BBLAST_TAC);
+
+val pl_compute = Q.store_thm("pl_compute",`
+  pl (w1:word32) (w2:word32) =
+  if w1 = NEG_INF ∨ w2 = NEG_INF then NEG_INF
+  else
+  let s:word64 = sw2sw w1 + sw2sw w2 in
+  round_to_inf s`,
+  rw[pl_def]>>fs[round_to_inf_def]>>
+  rpt (pop_assum mp_tac)>> EVAL_TAC>>
+  rw[]>>
+  blastLib.FULL_BBLAST_TAC)
+
+val wtimes_compute = Q.store_thm("wtimes_compute",`
+  wtimes w1 w2 =
+  let prod = sw2sw w1 * sw2sw w2 in round_to_inf prod`,
+  EVAL_TAC>>rw[]>>
+  rpt(pop_assum mp_tac)>> EVAL_TAC>>
+  blastLib.FULL_BBLAST_TAC);
 
 (* Free variables *)
 val fv_trm_def = Define`
@@ -245,7 +460,8 @@ val fv_trm_def = Define`
   (fv_trm (Times t1 t2) = fv_trm t1 ++ fv_trm t2) ∧
   (fv_trm (Max t1 t2) = fv_trm t1 ++ fv_trm t2) ∧
   (fv_trm (Min t1 t2) = fv_trm t1 ++ fv_trm t2) ∧
-  (fv_trm (Neg t) = fv_trm t)`
+  (fv_trm (Neg t) = fv_trm t) ∧
+  (fv_trm (Abs t) = fv_trm t)`
 
 val fv_fml_def = Define`
   (fv_fml (Le t1 t2) = fv_trm t1 ++ fv_trm t2) ∧
@@ -259,8 +475,8 @@ val fv_fml_def = Define`
 val fv_trm_coincide = Q.store_thm("fv_trm_coincide",`
   ∀t w v.
   EVERY (λx. ALOOKUP w x = ALOOKUP v x) (fv_trm t) ⇒
-  wtsem t w = wtsem t v`,
-  Induct>>fs[fv_trm_def,wtsem_def,lookup_var_def]>>rw[]>>
+  cwtsem t w = cwtsem t v`,
+  Induct>>fs[fv_trm_def,cwtsem_def,lookup_var_def]>>rw[]>>
   rpt(pairarg_tac>>fs[])>>
   metis_tac[PAIR,FST,SND]);
 
@@ -268,8 +484,8 @@ val fv_trm_coincide = Q.store_thm("fv_trm_coincide",`
 val fv_fml_coincide = Q.store_thm("fv_fml_coincide",`
   ∀f w v.
   EVERY (λx. ALOOKUP w x = ALOOKUP v x) (fv_fml f) ⇒
-  wfsem f w = wfsem f v`,
-  Induct>>fs[fv_fml_def,wfsem_def]>>rw[]>>
+  cwfsem f w = cwfsem f v`,
+  Induct>>fs[fv_fml_def,cwfsem_def]>>rw[]>>
   rpt(pairarg_tac>>fs[])>>rw[]>>
   metis_tac[PAIR,FST,SND,fv_trm_coincide]);
 
@@ -281,14 +497,14 @@ val AssignAnyPar_def = Define`
 val AssignAnyPar_sem = Q.store_thm("AssignAnyPar_sem",`
   ∀xs ws w w'.
   ALL_DISTINCT xs ==>
-  (wpsem (AssignAnyPar xs) w w' ⇔
+  (cwpsem (AssignAnyPar xs) w w' ⇔
   ∃ws.
   LENGTH ws = LENGTH xs ∧
   EVERY (λ(a,b). a ≤ b) ws ∧
   w' = (REVERSE (ZIP(xs,ws)) ++ w))`,
   Induct>>rw[AssignAnyPar_def]>>
-  simp[Once wpsem_cases]>>
-  simp[Once wpsem_cases,PULL_EXISTS]>>
+  simp[Once cwpsem_cases]>>
+  simp[Once cwpsem_cases,PULL_EXISTS]>>
   rw[EQ_IMP_THM]
   >-
     (qexists_tac`(a,b)::ws`>>simp[])
@@ -324,19 +540,19 @@ val AssignPar_sem = Q.store_thm("AssignPar_sem",`
   ALL_DISTINCT ls ∧
   no_overlap ls (FLAT (MAP fv_trm rs)) ∧
   LENGTH ls = LENGTH rs ⇒
-  (wpsem (AssignPar ls rs) w w' ⇔
-  w' = REVERSE (ZIP(ls, MAP (λr. wtsem r w) rs)) ++ w)`,
+  (cwpsem (AssignPar ls rs) w w' ⇔
+  w' = REVERSE (ZIP(ls, MAP (λr. cwtsem r w) rs)) ++ w)`,
   simp[Once no_overlap_sym]>>
   Induct>>rw[AssignPar_def]
   >-
-    simp[Once wpsem_cases]
+    simp[Once cwpsem_cases]
   >>
   Cases_on`rs`>>fs[AssignPar_def]>>
-  simp[Once wpsem_cases]>>
-  simp[Once wpsem_cases]>>
+  simp[Once cwpsem_cases]>>
+  simp[Once cwpsem_cases]>>
   first_x_assum(qspec_then`t` mp_tac)>>
   simp[]>>
-  disch_then(qspecl_then [`(h,wtsem h' w):: w`,`w'`] mp_tac)>>
+  disch_then(qspecl_then [`(h,cwtsem h' w):: w`,`w'`] mp_tac)>>
   impl_tac>-
     fs[no_overlap_thm]>>
   rw[]>>
@@ -356,11 +572,11 @@ val AssignVarPar_sem = Q.store_thm("AssignVarPar_sem",`
   ALL_DISTINCT ls ∧
   no_overlap ls rs ∧
   LENGTH ls = LENGTH rs ⇒
-  (wpsem (AssignVarPar ls rs) w w' ⇔
+  (cwpsem (AssignVarPar ls rs) w w' ⇔
   w' = REVERSE (ZIP(ls, MAP (lookup_var w) rs)) ++ w)`,
   rw[AssignVarPar_def]>>
-  `MAP (lookup_var w) rs = MAP (λr. wtsem r w) (MAP Var rs)` by
-     simp[MAP_EQ_f,MAP_MAP_o,wtsem_def]>>
+  `MAP (lookup_var w) rs = MAP (λr. cwtsem r w) (MAP Var rs)` by
+     simp[MAP_EQ_f,MAP_MAP_o,cwtsem_def]>>
   rw[]>>
   match_mp_tac AssignPar_sem>>
   fs[MAP_MAP_o,fv_trm_def,o_DEF,FLAT_MAP_SING]);
@@ -370,8 +586,7 @@ val AssignVarPar_imp = Q.store_thm("AssignVarPar_imp",`
   ALL_DISTINCT ls ∧
   no_overlap ls rs ∧
   LENGTH ls = LENGTH rs ⇒
-  wpsem (AssignVarPar ls rs) w (REVERSE (ZIP(ls, MAP (lookup_var w) rs)) ++ w)`,
+  cwpsem (AssignVarPar ls rs) w (REVERSE (ZIP(ls, MAP (lookup_var w) rs)) ++ w)`,
   metis_tac[AssignVarPar_sem]);
-
 
 val _ = export_theory();
